working on demo

test/Demo.v
@@ -11,14 +11,14 @@ Fixpoint max_spec (a b : nat) :=
 
 (* max of 2 nats using recursors *)
 (* language that Oeuf currently understands *)
-Definition max (a b : nat) :=
+Definition max (a b : nat) : nat :=
   @nat_rect (fun _ => nat -> nat)
             (fun base => base) (* if a is 0, return b *)
-            (fun a' IHa => (* if a is S a', *)
-               @nat_rect (fun _ => nat)
+            (fun a' IHa b => (* if a is S a', *)
+               (@nat_rect (fun _ => nat)
                          (S a') (* if b is 0, return S a' *)
-                         (fun b' IHignore => S (IHa b')) (* if b is S b', recurse *)
-            )
+                         (fun b' IHignore => S (IHa b'))) b) (* if b is S b', recurse *)
+            
             a b.
 
 (* prove to ourselves that they're the same *)
@@ -44,17 +44,19 @@ Definition max_list_spec (l : list nat) : nat :=
 
 (* max of a list of nats using recursors *)
 (* language that Oeuf reflection currently understands *)
-Definition max_list_h (l : list nat) :=
+Definition max_list_h (l : list nat) (cur : nat) : nat :=
   @list_rect nat
              (fun _ => nat -> nat)
              (fun cur => cur)
              (fun f r IHl cur =>
                 let cur' := max cur f in
-                IHl cur') l.
+                IHl cur') l cur.
 
-Definition max_list (l : list nat) :=
+(* wrapper to use helper function *)
+Definition max_list (l : list nat) : nat :=
   max_list_h l 0.
 
+(* helper lemma *)
 Lemma same_max_list_h :
   forall l x,
     max_list_helper l x = max_list_h l x.
@@ -62,6 +64,7 @@ Proof.
   induction l; intros; unfold max_list_helper; unfold max_list_h; simpl; eauto.
 Qed.
 
+(* prove that impl is same as spec *)
 Lemma same_max_list :
   forall l,
     max_list_spec l = max_list l.
@@ -74,19 +77,22 @@ Require Pretty CompilationUnit.
 Require Import SourceLang.
 Require OeufPlugin.OeufPlugin.
   
-  (* get our representation of the type of max *)
-  Definition max_reflect_ty : type :=
-    ltac:(type_reflect (nat -> nat -> nat)).
+    (* get our representation of the type of max_list *)
+  Definition max_list_reflect_ty : type :=
+    ltac:(type_reflect (list nat -> nat)).
 
   (* get the UNTRUSTED reflection of add *)
-  Definition max_reflect {l} : expr l max_reflect_ty :=
-    ltac:(let x := eval unfold max in max in reflect x).
+  Definition max_list_reflect {l} : expr l max_list_reflect_ty :=
+    ltac:(let x := eval unfold max_list in max_list in (* no separate compilation *)
+              let y := eval unfold max_list_h in x in (* have to unfold everything *)
+                  let z := eval unfold max in y in (* even max *)
+              reflect z).
 
   (* use translation validation to prove our add reflection is correct *)
-  Example max_reflect_correct : forall l h, expr_denote(l := l) max_reflect h = add.
+  Example max_list_reflect_correct : forall l h, expr_denote(l := l) max_list_reflect h = max_list.
   Proof. reflexivity. Qed.
 
 (* write our reflection to file "max.oeuf" *)
-Eval compute Then Write To File "max.oeuf"
+Oeuf Eval compute Then Write To File "max_list.oeuf"
      (Pretty.compilation_unit.print
-        (CompilationUnit.singleton (max_reflect) "max")).
+        (CompilationUnit.singleton (max_list_reflect) "max_list")).
